coq/well-scoped/sn.v
@@ -1,59 +1,58 @@
 (** * Proof of Strong Normalisation *)
 
-From mathcomp Require Import ssreflect.all_ssreflect.
-Require Import axioms fintype graded stlc ARS.
+Require Import axioms fintype stlc ARS.
 Set Implicit Arguments.
 Unset Strict Implicit.
 
-(** This is a simple implementation of the rewriting technique of Autosubst. *)
-Local Ltac asimpl :=
-  repeat progress (cbn; fsimpl; gsimpl; tm_simpl).
 Ltac inv H := inversion H; subst; clear H.
+Notation "M .[ sigma ]'" := (ren_tm sigma M) (at level 60, format "M .[ sigma ]'").
+Notation "M .[ sigma ]" := (subst_tm sigma M) (at level 60, format "M .[ sigma ]").
 
 (** ** One-Step Reduction *)
 Inductive step {n} : tm n -> tm n -> Prop :=
-| step_beta (T : ty) (M : tm n.+1) (N : tm n) :
-    step (Tm.app (Tm.lam T M) N) M.[N .: Tm.var]%tm
+| step_beta (T : ty) (M : tm (S n)) (N : tm n) :
+    step (app (lam T M) N) (M.[N .: var_tm])
 | step_appL M N M' :
-    step M M' -> step (Tm.app M N) (Tm.app M' N)
+    step M M' -> step (app M N) (app M' N)
 | step_appR M N N' :
-    step N N' -> step (Tm.app M N) (Tm.app M N')
+    step N N' -> step (app M N) (app M N')
 | step_abs T M M' :
-    @step n.+1 M M' -> step (Tm.lam T M) (Tm.lam T M').
+    @step (S n) M M' -> step (lam T M) (lam T M').
 
 Lemma step_ebeta {n} T M N (M' : tm n) :
-  M' = M.[N .: Tm.var]%tm -> step (Tm.app (Tm.lam T M) N) M'.
-Proof. move->. exact: step_beta. Qed.
+  M' = M.[N .: var_tm] -> step (app (lam T M) N) M'.
+Proof. intros ->. apply step_beta. Qed.
 
 Module Reduction.
 Lemma substitutivity {n1 n2} (sigma : fin n1 -> tm n2) M M' :
-  step M M' -> step M.[sigma]%tm M'.[sigma]%tm.
+  step M M' -> step (M.[sigma]) (M'.[sigma]).
 Proof.
-  move=> H. elim: H n2 sigma => {n1 M M'}; asimpl; eauto using @step.
-  - move=> n1 T M M' n2 sigma. apply: step_ebeta. by asimpl.
+  intros H. revert n2 sigma. induction H; intros n2 sigma; asimpl; eauto using @step.
+  - apply step_ebeta. now asimpl.
 Qed.
 
-Lemma naturality m n (M: tm m) (rho: fin m -> fin n) M' :
-  step (M ◁ rho)%tm M' -> exists M'', step M M'' /\ M' = (M'' ◁ rho)%tm.
+Lemma naturality m n (M: tm m) (rho: fin m -> fin n) N :
+  step (M.[rho]') N -> exists N', step M N' /\ N = (ren_tm rho N').
 Proof.
-  elim: M n rho M' => {m}.
-  - move=>m x n rho M H. inv H.
-  - move=>m M1 IHM1 M2 IHM2 n rho M H. inv H.
-    + assert (exists s1', M1 = Tm.lam T s1' ) as [s1' B].
+  revert n N rho. induction M as [m x | m M1 IHM1 M2 IHM2 | m T M IHM]; intros n N rho H.
+  - inv H.
+  - inv H.
+    + assert (exists s1', M1 = lam T s1' ) as [s1' B].
       { destruct M1; simpl in *; try congruence; eauto. inversion H1. subst. eauto. }
       subst.
-      exists (s1'.[M2 .: Tm.var])%tm. split.
+      exists (s1'.[M2 .: var_tm]). split.
       * constructor.
       * revert H1. asimpl. intros H1. inv H1. asimpl. reflexivity.
     + destruct (IHM1 _ _ _ H3) as (M1'&IH11&IH12). subst.
-      exists (Tm.app M1' M2). split. constructor. assumption.
+      exists (app M1' M2). split. constructor. assumption.
       reflexivity.
     + destruct (IHM2 _ _ _ H3) as (M2'&IH21&IH22).
-      subst. exists (Tm.app M1 M2').  split. now constructor. reflexivity.
-  - move => m S M IHM n rho T H. inv H.
+      subst. exists (app M1 M2').  split. now constructor. reflexivity.
+  - inv H.
     destruct (IHM _ _ _ H3) as (N'&IH1&->).
-    exists (Tm.lam S N'). split=>//. by apply: step_abs.
+    exists (lam T N'). split. now apply step_abs. reflexivity.
 Qed.
+
 End Reduction.
 
 (** ** Many-Step Reduction *)
@@ -64,32 +63,33 @@ Definition sred {n k} (sigma tau : fin n -> tm k) :=
 
 Module ManyStepReduction.
 Lemma red_app {n} (M M' N N' : tm n) :
-  red M M' -> red N N' -> red (Tm.app M N) (Tm.app M' N').
+  red M M' -> red N N' -> red (app M N) (app M' N').
 Proof.
-  move=> T B. apply: (star_trans (Tm.app M' N)).
-  - apply: (star_hom (@Tm.app n^~ N)) T => x y. exact: step_appL.
-  - apply: star_hom B => x y. exact: step_appR.
+  intros T B. apply (star_trans (app M' N)).
+  - eapply (star_hom (fun M => @app n M N)); [|eauto].
+    + intros. eapply step_appL; exact H.
+  - eapply star_hom; [|eauto]. eauto using step_appR.
 Qed.
 
-Lemma red_abs {n} T (M M' : tm n.+1) :
-  red M M' -> red (Tm.lam T M) (Tm.lam T M').
-Proof. apply: star_hom => x y. exact: step_abs. Qed.
+Lemma red_abs {n} T (M M' : tm (S n)) :
+  red M M' -> red (lam T M) (lam T M').
+Proof. apply star_hom. eauto using step_abs. Qed.
 
 Lemma red_inst {n1 n2} (f : fin n1 -> tm n2) s t :
-  red s t -> red s.[f]%tm t.[f]%tm.
-Proof. apply: star_hom => x y. exact: Reduction.substitutivity. Qed.
+  red s t -> red (s.[f]) (t.[f]).
+Proof. apply star_hom. eauto using Reduction.substitutivity. Qed.
 
 Lemma red_compat {n1 n2} (f1 f2 : fin n1 -> tm n2) s :
-  sred f1 f2 -> red s.[f1]%tm s.[f2]%tm.
+  sred f1 f2 -> red (s.[f1]) (s.[f2]).
 Proof.
-  elim: s n2 f1 f2; intros; asimpl; eauto using red_app,red_abs.
-  - apply: red_abs. apply: H. hnf=>/= -[i|]//=. asimpl. rewrite Tm.embed [(_ ◁ (_))%tm]Tm.embed.
-    apply: red_inst. exact: H0.
+  revert n2 f1 f2; induction s; intros n2 f1 f2 H; asimpl; eauto using red_app, red_abs.
+  - apply red_abs, IHs. intros [i|]; [|constructor].
+    apply red_inst, H.
 Qed.
 
 Lemma red_beta {n} s (N N' : tm n) :
-  step N N' -> red s.[N .: Tm.var]%tm s.[N' .: Tm.var]%tm.
-Proof. move=> h. apply: red_compat => /=-[i|]/=; [exact: starR|exact: star1]. Qed.
+  step N N' -> red (s.[N .: var_tm]) (s.[N' .: var_tm]).
+Proof. intros h. apply red_compat. intros [i|]; [now apply starR|now apply star1]. Qed.
 
 End ManyStepReduction.
 Import ManyStepReduction.
@@ -98,62 +98,62 @@ Import ManyStepReduction.
 Notation sn := (sn (@step _)).
 Module SN.
 Lemma closed_app {n} (t s : tm n) :
-  sn (Tm.app s t) -> sn s.
-Proof. apply: (sn_preimage (h := @Tm.app n^~t)) => x y. exact: step_appL. Qed.
+  sn (app s t) -> sn s.
+Proof. apply (sn_preimage (h := fun M => @app n M t)). eauto using step_appL. Qed.
 
 Lemma substitutivity {n1 n2} (f : fin n1 -> tm n2) s :
-  sn s.[f]%tm -> sn s.
-Proof. apply: sn_preimage. exact: Reduction.substitutivity. Qed.
+  sn (s.[f]) -> sn s.
+Proof. apply sn_preimage. apply Reduction.substitutivity. Qed.
 
 (** *** Lemma 2.4 - SN Closure under Weakening *)
 Lemma weak k (M: tm k) k' (rho : fin k -> fin k'):
-  sn M -> sn (M ◁ rho)%tm.
+  sn M -> sn (M .[rho]').
 Proof.
-  move=> H. move: k' rho. elim: H => x H IH k' rho.
-  apply: SNI. move => x' A.
+  intros H. revert k' rho. induction H as [x H IH]; intros k' rho.
+  apply SNI. intros x' A.
   destruct (Reduction.naturality A) as (x''&B1&B2); subst.
-  by apply: IH.
+  now apply IH.
 Qed.
 End SN.
 
 (** ** Syntactic typing *)
 Definition ctx n := fin n -> ty.
 Inductive has_type {n} (Gamma : ctx n) : tm n -> ty -> Prop :=
-| ty_var (x : fin n) :
-    has_type Gamma (Tm.var x) (Gamma x)
-| ty_abs (T S : ty) (M : tm n.+1) :
-    @has_type n.+1 (T .: Gamma) M S ->
-    has_type Gamma (Tm.lam T M) (arr T S)
+| ty_var_tm (x : fin n) :
+    has_type Gamma (var_tm x) (Gamma x)
+| ty_abs (S1 S2 : ty) (M : tm (S n)) :
+    @has_type (S n) (S1 .: Gamma) M S2 ->
+    has_type Gamma (lam S1 M) (arr S1 S2)
 | ty_app (T S : ty) (M N : tm n) :
     has_type Gamma M (arr T S) ->
     has_type Gamma N T ->
-    has_type Gamma (Tm.app M N) S.
-Notation "Gamma |- M :' T" := (has_type Gamma M T) (at level 20).
+    has_type Gamma (app M N) S.
+Notation "Gamma |- M : T" := (has_type Gamma M T) (at level 20, M at level 99).
 Definition ltc {k k'} (Gamma: ctx k) (Delta: ctx k') rho := forall x, Delta (rho x) = Gamma x.
 
 Module Typing.
 Lemma typing_ren n k (Gamma: ctx n) (Delta: ctx k) (rho: fin n -> fin k) (M: tm n) T :
-  ltc Gamma Delta rho  -> Gamma |- M :' T ->  Delta |- (M ◁ rho)%tm :' T.
+  ltc Gamma Delta rho  -> Gamma |- M : T ->  Delta |- (M .[rho]') : T.
 Proof.
-  move => H B. elim: B k rho Delta H  => {n Gamma M T} n Gamma; [move => x|move => S T M A IH |move =>S T M N A IHA B IHB]; move => k rho Delta H.
-  - rewrite -H. apply: ty_var.
-  - asimpl. apply: ty_abs. apply: IH.
-    move=> [x|] //. asimpl. apply: H.
-  - apply: ty_app; [exact: IHA _ _ H| exact: IHB _ _ H].
+  intros H B. revert k rho Delta H. induction B as [x | n Gamma T1 T2 M A IH | n Gamma T1 T2 M N A IHA B IHB]; intros k rho Delta H.
+  - rewrite <- H. apply ty_var_tm.
+  - apply ty_abs. apply IH.
+    intros [x|]; [|constructor]. asimpl. apply H.
+  - eapply ty_app; eauto.
 Qed.
 
 Lemma typing_inst n k (Gamma: ctx n) (Delta: ctx k) (sigma: fin n -> tm k) (M: tm n) T :
-  (forall x, Delta |- sigma x :' Gamma x) -> Gamma |- M :' T ->  Delta |- (M.[sigma])%tm :' T.
+  (forall x, Delta |- sigma x : Gamma x) -> Gamma |- M : T ->  Delta |- (M.[sigma]) : T.
 Proof.
-  move => A B. elim: B k sigma Delta A => {n Gamma M T} n Gamma; [move => x|move => S T M A IH |move =>S T M N A IHA B IHB]; move => k sigma Delta H.
-  - apply: H.
-  - asimpl. apply: ty_abs. apply: IH.
-    move=> [x|]. asimpl. apply: typing_ren =>//. apply: ty_var.
-  - apply: ty_app; [exact: IHA _ _ H| exact: IHB _ _ H].
+  intros A B. revert k sigma Delta A.  induction B as [x | n Gamma T1 T2 M A IH | n Gamma T1 T2 M N A IHA B IHB]; intros k sigma Delta H.
+  - apply H.
+  - apply ty_abs. apply IH.
+    intros [x|]; [|constructor]. eapply typing_ren; [intros y; reflexivity|apply H].
+  - apply ty_app with (T := T1); eauto.
 Qed.
 
 Lemma step_typing k (Gamma: ctx k) M T :
-  Gamma |- M :' T -> forall M', step M M' -> Gamma |- M' :' T.
+  Gamma |- M : T -> forall M', step M M' -> Gamma |- M' : T.
 Proof.
   induction 1 as [k Gamma x | k Gamma T S M A IHA | k Gamma T S M N A IHA B IHB]; intros M' H; cbn.
   - inv H.
@@ -161,10 +161,10 @@ Proof.
   - inv H.
     + inv A. eapply typing_inst; try eassumption.
       intros [i|]; [econstructor | assumption].
-    + apply: ty_app. by apply: IHA. by [].
-    + apply: ty_app.
-      * exact: A.
-      * by apply: IHB.
+    + eapply ty_app. now apply IHA. assumption.
+    + eapply ty_app.
+      * exact A.
+      * now apply IHB.
 Qed.
 End Typing.
 Import Typing.
@@ -175,14 +175,14 @@ Definition cand n := tm n -> Prop.
 
 Fixpoint L {k} (Gamma: ctx k) (T: ty) : cand k :=
   match T with
-  |Base => fun M => Gamma |- M :' T /\ sn M
-  |arr T1 T2 => fun M => Gamma |- M :' arr T1 T2 /\
-                     (forall k' (N: tm k') (Delta: ctx k') rho, ltc Gamma Delta rho -> L Delta T1 N -> L Delta T2 (Tm.app (M ◁ rho)%tm N))
+  |Base => fun M => Gamma |- M : T /\ sn M
+  |arr T1 T2 => fun M => Gamma |- M : arr T1 T2 /\
+                     (forall k' (N: tm k') (Delta: ctx k') rho, ltc Gamma Delta rho -> L Delta T1 N -> L Delta T2 (app (M.[rho]') N))
   end.
 
 Lemma L_typing {k} (Gamma: ctx k) (T: ty) M :
-  L Gamma T M -> Gamma |- M :' T.
-Proof. move=> H. destruct T; simpl in *; intuition. Qed.
+  L Gamma T M -> Gamma |- M : T.
+Proof. intros H. destruct T; simpl in *; intuition. Qed.
 
 Module L.
 
@@ -195,55 +195,57 @@ Proof.
     + inv H2. now apply H.
   - split; [|].
     + eapply step_typing; eassumption.
-    + intros k' N Delta rho H H0. apply IHS with (M := Tm.app (M ◁ rho)%tm N).
-      * econstructor. rewrite Tm.embed. rewrite (Tm.embed _ _ M'). now apply Reduction.substitutivity.
-      * apply: H2 => //.
+    + intros k' N Delta rho H H0. apply IHS with (M := app (M.[rho]') N).
+      * econstructor. asimpl. now apply Reduction.substitutivity.
+      * now apply H2.
 Qed.
 
 Lemma preservation_red {k} (Gamma : ctx k) M M' T :
   red M M' -> L Gamma T M -> L Gamma T M'.
-Proof. move=> H. elim: H; eauto using preservation. Qed.
+Proof. intros H. induction H; eauto using preservation. Qed.
 
 Lemma ren k k' (Gamma: ctx k) (Delta: ctx k') rho M T (Gamma_Delta : ltc Gamma Delta rho):
-  L Gamma T M -> L Delta T (M ◁ rho)%tm.
+  L Gamma T M -> L Delta T (M .[rho]').
 Proof.
-  elim:T => [|T IHT S IHS] [H1 H2]; split; try apply typing_ren with (Gamma := Gamma) =>//.
+  induction T as [|T IHT S IHS]; intros [H1 H2]; split; try apply typing_ren with (Gamma := Gamma); eauto.
   - now apply SN.weak.
-  - move => k'' N Delta' rho' A1 A2. asimpl. apply H2 =>// i.
-    rewrite <- Gamma_Delta. now rewrite A1.
+  - intros k'' N Delta' rho' A1 A2.
+    assert ((M.[rho]').[rho']' = M.[rho >> rho']') as -> by (now asimpl).
+    apply H2; [|assumption].
+    + intros x. now rewrite <- Gamma_Delta, <- A1.
 Qed.
 
 Definition neutral k (M: tm k) :=
   match M with
-  |Tm.lam _ _ => False
+  |lam _ _ => False
   |_ => True
   end.
 
 (** Girard's theorem. *)
 Lemma Girard k (Gamma: ctx k) (M : tm k) T :
-  (L Gamma T M -> sn M) /\ (Gamma |- M :' T -> neutral M -> (forall N, step M N -> L Gamma T N) -> L Gamma T M).
+  (L Gamma T M -> sn M) /\ (Gamma |- M : T -> neutral M -> (forall N, step M N -> L Gamma T N) -> L Gamma T M).
 Proof.
-  revert k M Gamma. induction T as [|T IHT S IHS]; intros k M Gamma; simpl in *.
+  revert k M Gamma. induction T as [|T1 IHT1 T2 IHT2]; intros k M Gamma; simpl in *.
   - intuition. constructor. intros N H'. firstorder.
   - split.
     + intros [H1 H2].
-      have A:  L (T .: Gamma) S (Tm.app (M ◁ shift)%tm (Tm.var k.+1 None)).
-      { apply H2 => //. apply IHT =>//. constructor. intros N H. inv H. }
-      rewrite Tm.embed in A.
-      now apply IHS, SN.closed_app, SN.substitutivity in A.
-    + intros H0 H1 H2. split =>//.
+      assert (A:  L (T1 .: Gamma) T2 (app (M .[shift]') (@var_tm (S k) None))).
+      { apply H2. intros x; reflexivity. apply IHT1. constructor. constructor. intros N H. inv H. }
+      erewrite rinst_inst_tm in A; [|reflexivity].
+      now eapply IHT2, SN.closed_app, SN.substitutivity in A.
+     + intros H0 H1 H2. split; [assumption |].
       intros k' N Delta rho H3 H4.
-      have SN_N : sn N by firstorder.
+      assert ( SN_N : sn N) by firstorder.
       induction SN_N as [N sn_N IHN].
-      apply IHS =>//.
-      * rewrite Tm.embed. eapply ty_app.
-        -- eapply typing_inst; try eassumption.
-           intros x =>/=. rewrite <- H3. constructor.
-        -- auto using L_typing.
+      apply IHT2; try constructor.
+       * erewrite rinst_inst_tm; [|reflexivity]. eapply ty_app.
+         -- eapply typing_inst; try eassumption.
+            intros x. rewrite <- H3. constructor.
+         -- auto using L_typing.
       * intros M' A. inv A.
         -- destruct M; simpl in *; try congruence. contradiction.
         -- destruct (Reduction.naturality H7) as [M'' [H' ->]]. now apply H2.
-        -- apply IHN =>//. eapply preservation; eassumption.
+        -- apply IHN; [assumption|]. eapply preservation; eassumption.
 Qed.
 
 Lemma sn k (Gamma: ctx k) (M : tm k) T:
@@ -252,9 +254,9 @@ Proof.
   intros H. eapply Girard. eassumption.
 Qed.
 
-Lemma var k (Gamma: ctx k) x :
-  L Gamma (Gamma x) (Tm.var k x).
-Proof. apply Girard =>//. apply: ty_var. move => N H. inv H. Qed.
+Lemma var_tm k (Gamma: ctx k) x :
+  L Gamma (Gamma x) (var_tm x).
+Proof. apply Girard; try constructor. intros N H. inv H. Qed.
 
 End L.
 
@@ -262,44 +264,48 @@ End L.
 
 Module StrongNormalisation.
 
-Lemma beta_closure k Gamma (N: tm k) T (N_ty : Gamma |- N :' T) :
-  sn N -> forall S M, (T .: Gamma) |- M :' S ->  L Gamma S (M.[N .: Tm.var])%tm -> L Gamma S (Tm.app (Tm.lam T M) N).
+Lemma beta_closure k Gamma (N: tm k) T (N_ty : Gamma |- N : T) :
+  sn N -> forall S M, (T .: Gamma) |- M : S ->  L Gamma S (M.[N .: var_tm]) -> L Gamma S (app (lam T M) N).
 Proof.
   induction 1 as [N H IH_N]. intros S M M_ty H'.
-  have sn_M := SN.substitutivity (L.sn H'). induction sn_M as [M sn_M IH_M].
-  apply L.Girard =>//.
-  - by repeat econstructor.
-  - intros M' H1. inv H1 =>//.
+  assert (sn_M := SN.substitutivity (L.sn H')). induction sn_M as [M sn_M IH_M].
+  apply L.Girard; try constructor.
+  - now repeat econstructor.
+  - intros M' H1. inv H1; try eauto.
     + inv H4. apply IH_M; eauto using step_typing, L.preservation, Reduction.substitutivity.
     + apply IH_N; eauto using step_typing, L.preservation_red, red_beta.
 Qed.
 
 Theorem fundamental_theorem k (Gamma: ctx k) M T :
-  Gamma |- M :' T -> forall k' (Gamma': ctx k') sigma,  (forall x,  L Gamma' (Gamma x) (sigma x)) -> L Gamma' T (M.[sigma])%tm.
+  Gamma |- M : T -> forall k' (Gamma': ctx k') sigma,  (forall x,  L Gamma' (Gamma x) (sigma x)) -> L Gamma' T (M.[sigma]).
 Proof.
-  induction 1 as [| k Gamma T S M H IH | k Gamma T S M N A IHA B IHB]; intros k' Gamma' sigma adm; asimpl.
+  induction 1 as [| k Gamma T1 T2 M H IH | k Gamma T1 T2 M N A IHA B IHB]; intros k' Gamma' sigma adm; asimpl.
   - apply adm.
-  - have M_ty :  (T .: Gamma') |- (M.[Tm.var k'.+1 bound .: sigma >> th1 shift])%tm :' S.
-    { have A: forall x, Gamma' |- sigma x :' Gamma x by auto using L_typing.
-      apply typing_inst with (Gamma := T .: Gamma) =>//.
-      intros [i|]; [|apply: ty_var]. asimpl. apply typing_ren with (Gamma := Gamma') =>//.  }
+  - assert ( M_ty :  (T1 .: Gamma') |- (M.[@var_tm (S k') bound .: sigma >> ren_tm shift]) : T2).
+    { assert (A: forall x, Gamma' |- sigma x : Gamma x) by auto using L_typing.
+      apply typing_inst with (Gamma := T1 .: Gamma); [|assumption].
+      intros [i|]; [|constructor].
+      -  apply typing_ren with (Gamma := Gamma'); try constructor. apply A. }
     split.
-    + now apply ty_abs.
+    + apply ty_abs. revert M_ty. asimpl. auto.
     + intros k'0 N Delta rho A B.
       apply beta_closure; eauto using L_typing, L.sn.
-      * apply typing_ren with (Gamma := T .: Gamma'); [intros [i|]; simpl; congruence | assumption] .
+      * apply typing_ren with (Gamma := T1 .: Gamma'); [intros [i|]; simpl; congruence | ]. revert M_ty. now asimpl.
       * asimpl. apply IH.
-        intros [i|] =>//=. rewrite <- Tm.embed. apply L.ren with (Gamma := Gamma') =>//.
+        intros [i|]; [|assumption].
+        -- unfold up_ren. fsimpl. simpl. unfold funcomp. erewrite <- rinst_inst_tm; [|reflexivity].
+           eapply L.ren. apply A. apply adm.
   - destruct (IHA _ _ _ adm) as [IHA1 IHA2]. specialize (IHB _ _ _ adm).
-    have -> : (M.[sigma])%tm = ((M.[sigma])%tm ◁ id)%tm by now asimpl.
-    now apply IHA2.
+    assert ((M.[sigma]) = ((M.[sigma]).[idren]')) as -> by now asimpl.
+    apply IHA2; unfold ltc; auto.
 Qed.
 
+
 Corollary strong_normalisation k (Gamma: ctx k) M T :
-  Gamma |- M :' T -> sn M.
+  Gamma |- M : T -> sn M.
 Proof.
   intros A. apply L.sn with (Gamma := Gamma) (T := T).
-  enough (H: L Gamma T  (M.[Tm.var])%tm) by now (revert H; asimpl).
-  apply fundamental_theorem with (Gamma := Gamma); auto using L.var.
+  enough (H: L Gamma T  (M.[var_tm])) by now (revert H; asimpl).
+  apply fundamental_theorem with (Gamma := Gamma); auto using L.var_tm.
 Qed.
 End StrongNormalisation.
