coq/well-typed/stlc.v
@@ -1,4 +1,5 @@
 Require Import base contexts.
+Opaque at_ty.
 
 Inductive tm (G : ctx) : ty -> Type :=
 | var A : at_ty G A -> tm G A
@@ -14,9 +15,9 @@ Definition subst (G1 G2 : ctx) := env G1 (tm G2).
 
 Fixpoint rinst {G1 G2} (f : ren G1 G2) {A} (s : tm G1 A) : tm G2 A :=
   match s with
-  | var _ i => var (f _ i)
-  | app _ _ s t => app (rinst f s) (rinst f t)
-  | lam _ _ b => lam (rinst (var0 .: (f >> shift)) b)
+  | var i => var (f _ i)
+  | app s t => app (rinst f s) (rinst f t)
+  | lam b => lam (rinst (var0 .: (f >> shift)) b)
   end.
 
 Definition up {G1 G2 A} (f : subst G1 G2) : subst (A :: G1) (A :: G2) :=
@@ -24,9 +25,9 @@ Definition up {G1 G2 A} (f : subst G1 G2) : subst (A :: G1) (A :: G2) :=
 
 Fixpoint inst {G1 G2} (f : subst G1 G2) {A} (s : tm G1 A) : tm G2 A :=
   match s with
-  | var _ i => f _ i
-  | app _ _ s t => app (inst f s) (inst f t)
-  | lam _ _ b => lam (inst (up f) b)
+  | var i => f _ i
+  | app s t => app (inst f s) (inst f t)
+  | lam b => lam (inst (up f) b)
   end.
 
 (** ** Identity instantiation *)
@@ -36,61 +37,59 @@ Definition ids {G} : subst G G := @var G.
 Lemma rinst_idren {G A} (s : tm G A) :
   rinst idren s = s.
 Proof.
-  elim: s => {G A}[//|G A B s ihs t iht|G A B s ihs] /=;
-                 intros; simpl; subst; try congruence.
-  - fsimpl. by rewrite ihs.
+  induction s; intros; try reflexivity; try (simpl; subst; congruence); simpl.
+  - fsimpl. congruence.
 Qed.
 
 Lemma rinst_inst {G1 G2} (f : ren G1 G2) :
   @rinst G1 G2 f = @inst G1 G2 (f >> ids).
 Proof.
-  fext. intros A s.
-  elim: s G2 f => {G1 A}[//|G1 A B s ihs t iht|G1 A B s ihs]/= G2 f; intros; simpl; subst; try congruence.
-  - rewrite ihs /up. by fsimpl.
+  fext. intros A s. revert G2 f.
+  induction s; intros; simpl; subst; try reflexivity; try congruence.
+  - unfold up. rewrite IHs. now fsimpl.
 Qed.
 
 Lemma inst_ids {G A} (s : tm G A) :
   inst ids s = s.
-Proof.
-  by rewrite -{2}[s]rinst_idren rinst_inst.
-Qed.
+Proof. now rewrite <- rinst_idren, rinst_inst. Qed.
 
 (** ** Composition of instantiations *)
 
 Lemma inst_rinst_comp {G1 G2 G3 A} (f : ren G1 G2) (g : subst G2 G3) (s : tm G1 A) :
   inst g (rinst f s) = inst (f >> g) s.
 Proof.
-  elim: s G2 G3 f g => {G1 A} [G1 A i|G1 A B s ihs t iht|G1 A B s ihs] G2 G3 f g //=.
-  - by rewrite ihs iht.
-  - rewrite ihs /up. by fsimpl.
+  revert G2 G3 f g.
+  induction s; intros; cbn; try reflexivity; try congruence.
+  - unfold up. rewrite IHs. now fsimpl.
 Qed.
 
 Lemma rinst_comp {G1 G2 G3 A} (f : ren G1 G2) (g : ren G2 G3) (s : tm G1 A) :
   rinst g (rinst f s) = rinst (f >> g) s.
 Proof.
-  by rewrite rinst_inst inst_rinst_comp rinst_inst.
+  now rewrite rinst_inst, inst_rinst_comp, rinst_inst.
 Qed.
 
 Lemma rinst_inst_comp {G1 G2 G3 A} (f : subst G1 G2) (g : ren G2 G3) (s : tm G1 A) :
   rinst g (inst f s) = inst (f >> @rinst _ _ g) s.
 Proof.
-  elim: s G2 G3 f g => {G1 A} [G1 A i|G1 A B s ihs t iht|G1 A B s ihs] G2 G3 f g //=; intros; simpl; subst; try congruence.
-  - rewrite ihs. do 2 f_equal. fext=> {B s ihs} B /=-[E|i]; first by destruct E.
-    rewrite/up/scomp/=. by rewrite !rinst_comp.
+  revert G2 G3 f g.
+  induction s; intros; simpl; subst; try congruence; try reflexivity.
+  - unfold up, scomp. rewrite IHs. do 2 f_equal. fext. intros C [-> |i]; [reflexivity|].
+    unfold scomp. simpl. now rewrite !rinst_comp.
 Qed.
 
 Lemma up_comp {G1 G2 G3 A} (f : subst G1 G2) (g : subst G2 G3) :
   @up G1 G2 A f >> @inst _ _ (up g) = up (f >> @inst _ _ g).
 Proof.
-  fext=> B /=-[E|i]; first by destruct E. rewrite/up/scomp/=.
-  by rewrite rinst_inst_comp inst_rinst_comp.
+  fext. intros B [->|i]; [reflexivity|]. unfold up, scomp.
+  cbn. now rewrite rinst_inst_comp, inst_rinst_comp.
 Qed.
 
 Lemma inst_comp {G1 G2 G3 A} (f : subst G1 G2) (g : subst G2 G3) (s : tm G1 A) :
   inst g (inst f s) = inst (f >> @inst _ _ g) s.
 Proof.
-  elim: s G2 G3 f g => {G1 A} [G1 A i|G1 A B s ihs t iht|G1 A B s ihs] G2 G3 f g //=;  intros; simpl; subst; try congruence.
-  - by rewrite ihs up_comp.
+  revert G2 G3 f g. induction s as [G1 A i|G1 A B s ihs t iht|G1 A B s ihs]; intros; simpl; subst; try congruence; try reflexivity.
+  - now rewrite ihs, up_comp.
 Qed.
 
 (* Automation comp *)
@@ -103,22 +102,22 @@ Lemma comp_idl g g' (xi: subst g g') :
 Proof. fext. intros A x. reflexivity. Qed.
 
 Lemma sconsS G P A hd tl : shift >> @scons G P A hd tl = tl.
-Proof. by []. Qed.
+Proof. reflexivity. Qed.
 
 (** ** Automation *)
 Lemma rinst_idrenE G : @rinst G G idren = (fun A x => x).
-Proof. fext=> A s. exact: rinst_idren. Qed.
+Proof. fext. intros A s. apply rinst_idren. Qed.
 
 Lemma inst_idsE G : @inst G G ids = (fun A x => x).
-Proof. fext=> A s. exact: inst_ids. Qed.
+Proof. fext. intros A s. apply inst_ids. Qed.
 
 Lemma inst_up_beta {G1 G2 A B} (f : subst G1 G2) (s : tm (B :: G1) A) t :
   inst (inst f t .: ids) (inst (up f) s) =
   inst f (inst (t .: ids) s).
 Proof.
-  rewrite !inst_comp. f_equal. fext=> C /=-[E|i]; first by destruct E.
-  fsimpl. cbn. by rewrite/scomp inst_rinst_comp inst_ids.
+  rewrite !inst_comp. f_equal. fext. intros C [->|i]; [reflexivity|].
+  fsimpl. cbn. unfold scomp. rewrite inst_rinst_comp. fsimpl. now rewrite inst_ids.
 Qed.
 
 Ltac asimpl :=
-  repeat first [progress rewrite ?comp_rinst_inst ?sconsS ?comp_idl ?rinst_idrenE ?inst_ids ?rinst_inst_comp ?inst_rinst_comp ?inst_comp /up|fsimpl].
+  repeat first [unfold up; progress rewrite ?comp_rinst_inst, ?sconsS,?comp_idl,?rinst_idrenE,?inst_ids,?rinst_inst_comp,?inst_rinst_comp,?inst_comp|fsimpl].
