coq/well-scoped/ARS.v
@@ -1,7 +1,6 @@
 (** * Abstract Reduction Systems
 
     Useful lemmas when working with small-step reduction relations. *)
-From mathcomp Require Import ssreflect.all_ssreflect.
 Set Implicit Arguments.
 Unset Strict Implicit.
 Unset Printing Implicit Defensive.
@@ -28,7 +27,7 @@ Lemma star1 x y : e x y -> star x y.
 Proof. now apply starSE. Qed.
 
 Lemma star_trans y x z : star x y -> star y z -> star x z.
-Proof. move=> A. elim=> //={z} y' z _. exact: starSE. Qed.
+Proof. intros A B. revert x A. induction B; eauto using starSE. Qed.
 
 End Definitions.
 
@@ -38,16 +37,12 @@ Arguments star_trans {T e} y {x z} A B.
 Lemma star_img T1 T2 (f : T1 -> T2) (e1 : Rel T1) e2 :
   (forall x y, e1 x y -> star e2 (f x) (f y)) ->
   (forall x y, star e1 x y -> star e2 (f x) (f y)).
-Proof.
-  move=> A x y. elim=> //=y' z _ B /A. exact: star_trans.
-Qed.
+Proof. intros A x y. induction 1; eauto using star_trans. Qed.
 
 Lemma star_hom T1 T2 (f : T1 -> T2) (e1 : Rel T1) (e2 : Rel T2) :
   (forall x y, e1 x y -> e2 (f x) (f y)) ->
   (forall x y, star e1 x y -> star e2 (f x) (f y)).
-Proof.
-  move=> A. apply: star_img => x y /A. exact: star1.
-Qed.
+Proof. intros A. apply star_img. eauto using star1. Qed.
 
 Arguments star_hom {T1 T2} f e1 {e2} A x y B.
 
@@ -59,6 +54,6 @@ Inductive sn T (e: Rel T) x : Prop :=
 Lemma sn_preimage {T1 T2} (R1 : Rel T1) (R2 : Rel T2) (h : T1 -> T2) x :
   (forall x y, R1 x y -> R2 (h x) (h y)) -> sn R2 (h x) -> sn R1 x.
 Proof.
-  move eqn:(h x) => v A B. elim: B h x A eqn => {v} v _ ih h x A eqn.
-  apply: SNI => y /A. rewrite eqn => /ih; eauto.
+  intros H H'. remember (h x) as eqn. revert x Heqeqn.
+  induction H'; intros. subst. apply SNI. eauto.
 Qed.
