coq/well-scoped/axioms.v
@@ -1,4 +1,10 @@
-(** * Functional and Propositional Extensionality *)
+(** * Axiomatic Assumptions
+    For our development, we have to extend Coq with two well known axiomatic assumptions, namely _functional extensionality_ and _propositional extensionality_. The latter entails _proof irrelevance_.
+*)
+
+(** ** Functional Extensionality
+    We import the axiom from the Coq Standard Library and derive a utility tactic to make the assumption practically usable.
+*)
 Require Import Coq.Logic.FunctionalExtensionality.
 Require Import Program.Tactics.
 
@@ -16,6 +22,9 @@ Ltac fext := nointr repeat (
      refine (@forall_extensionalityS _ _ _ _)); intro
   end).
 
+(** ** Propositional Extensionality
+    We state the axiom of _propositional extensionality_ directly and use it to prove _proof irrelevance_.
+*)
 Axiom pext : forall P Q : Prop, (P <-> Q) -> (P = Q).
 
 Lemma pi {P : Prop} (p q : P) : p = q.
