coq/well-typed-sums/reduction.v
@@ -24,54 +24,50 @@ Inductive step : forall {G A}, tm G A -> tm G A -> Prop :=
 Definition ImPred {T1 T2} (P : T1 -> Prop) (f : T1 -> T2) (y : T2) :=  exists2 x : T1, P x & f x = y.
 
 Notation "[ 'Pred' s | x 'in' P ]" :=
-  (ImPred (fun x => P) (fun x => s)) : form_scope.
+  (ImPred (fun x => P) (fun x => s)).
 Notation "x ∈ P" := (P x) (at level 30, only parsing).
 
 Ltac inv H := dependent destruction H.
 
 Lemma im_predI {T1 T2} (P : T1 -> Prop) (f : T1 -> T2) (x : T1) :
   P x -> f x ∈ [Pred f x' | x' in P x'].
-Proof. move=> px. by exists x. Qed.
+Proof. intros px. now exists x. Qed.
 
 Lemma step_weak {G1 G2 A} (f : ren G1 G2) (s : tm G1 A) (t : tm G2 A) :
   step (rinst f s) t -> t ∈ [Pred rinst f s' | s' in step s s'].
-Proof.
-  move=> st. dependent induction st.
-  - inv s => //. inv x. inv s1 => //. inv x.
-    rewrite !rinst_inst. fsimpl. rewrite inst_up_beta. rewrite -rinst_inst.
-    apply: im_predI. exact: step_beta.
-  - inv s => //. inv x. case: (IHst _ _ _ erefl) => {IHst} s' ih e.
-    exists (lam s'). by constructor. by rewrite -e.
-  - inv s => //. inv x. case: (IHst _ _ _ erefl) => {IHst} s' ih e.
-    exists (app s' s4). by constructor. by rewrite -e.
-  - inv s => //. inv x. case: (IHst _ _ _ erefl) => {IHst} s' ih e.
-    exists (app s1 s'). by constructor. by rewrite -e.
-  - inv s => //. inv x. case: (IHst _ _ _ erefl) => {IHst} s' ih e.
-    exists (inl s'). by constructor. by rewrite -e.
-  - inv s => //. inv x. case: (IHst _ _ _ erefl) => {IHst} s' ih e.
-    exists (inr s'). by constructor. by rewrite -e.
-  - inv s => //. inv x. case: (IHst _ _ _ erefl) => {IHst} s' ih e.
-    exists (orelim s' s4 s5). by constructor. by rewrite -e.
-  - inv s => //. inv x. case: (IHst _ _ _ erefl) => {IHst} s' ih e.
-    exists (orelim s1 s' s3). by constructor. by rewrite -e.
-  - inv s => //. inv x. case: (IHst _ _ _ erefl) => {IHst} s' ih e.
-    exists (orelim s1 s2 s'). by constructor. by rewrite -e.
-  - inv s => //. inv x. inv s1 => //. inv x.
-    rewrite !rinst_inst. fsimpl. rewrite inst_up_beta. rewrite -rinst_inst.
-    apply: im_predI. exact: step_caseL.
-  - inv s => //. inv x. inv s1 => //. inv x.
-    rewrite !rinst_inst. fsimpl. rewrite inst_up_beta. rewrite -rinst_inst.
-    apply: im_predI. exact: step_caseR.
+Proof with simpl in *; try congruence.
+  intros st. dependent induction st.
+  - inv s... inv s1; try inv x... asimpl.
+    eexists. constructor. now asimpl.
+  - inv s... inv x. destruct (IHst _ _ _ eq_refl) as [s' ih <-].
+    exists (lam s'). now constructor. now fsimpl.
+  - inv s... inv x. destruct (IHst _ _ _ eq_refl) as [s' ih <-].
+    exists (app s' s4). now constructor. now fsimpl.
+  - inv s... inv x. destruct (IHst _ _ _ eq_refl) as [s' ih <-].
+    exists (app s1 s'). now constructor. now fsimpl.
+  - inv s... inv x. destruct (IHst _ _ _ eq_refl) as [s' ih <-].
+    exists (inl s'). now constructor. now fsimpl.
+  - inv s... inv x. destruct (IHst _ _ _ eq_refl) as [s' ih <-].
+    exists (inr s'). now constructor. now fsimpl.
+  - inv s... inv x. destruct (IHst _ _ _ eq_refl) as [s' ih <-].
+    exists (orelim s' s4 s5). now constructor. now fsimpl.
+  - inv s... inv x. destruct (IHst _ _ _ eq_refl) as [s' ih <-].
+    exists (orelim s1 s' s3). now constructor. now fsimpl.
+  - inv s... inv x. destruct (IHst _ _ _ eq_refl) as [s' ih <-].
+    exists (orelim s1 s2 s'). now constructor. now fsimpl.
+  - inv s... inv x. inv s1... inv x. asimpl.
+    eexists. now apply step_caseL. now asimpl.
+  - inv s... inv x. inv s1... inv x.
+    eexists. now apply step_caseR. now asimpl.
 Qed.
 
 Lemma step_inst {G1 G2 A} (f : subst G1 G2) (s t : tm G1 A) :
   step s t -> step (inst f s) (inst f t).
 Proof.
-  move=> st. elim: st G2 f => {G1 A s t}
-    [G1 A B b t|G1 A B b1 b2 _ ih|G1 A B s1 s2 t _ ih|G1 A B s t1 t2 _ ih|G1 A B s1 s2 _ ih|G1 A B s1 s2 _ ih|G1 A B C s1 s2 t u _ ih|G1 A B C s t1 t2 u _ ih|G1 A B C s t u1 u2 _ ih|G1 A B C s t u|G1 A B C s t u] G2 f/=; try (constructor; exact:ih).
-  - rewrite -inst_up_beta. exact: step_beta.
-  - rewrite -inst_up_beta. exact: step_caseL.
-  - rewrite -inst_up_beta. exact: step_caseR.
+  intros st. revert G2 f. induction st as  [G1 A B b t|G1 A B b1 b2 _ ih|G1 A B s1 s2 t _ ih|G1 A B s t1 t2 _ ih|G1 A B s1 s2 _ ih|G1 A B s1 s2 _ ih|G1 A B C s1 s2 t u _ ih|G1 A B C s t1 t2 u _ ih|G1 A B C s t u1 u2 _ ih|G1 A B C s t u|G1 A B C s t u]; intros G2 f; cbn; try (constructor; apply ih).
+  - rewrite <- inst_up_beta. apply step_beta.
+  - rewrite <- inst_up_beta. apply step_caseL.
+  - rewrite <- inst_up_beta. apply step_caseR.
 Qed.
 
 (** ** Multi-step reduction *)
@@ -82,18 +78,16 @@ Hint Resolve mstep_refl.
 
 Lemma mstep_trans G A (s t u : tm G A) :
   mstep s t -> mstep t u -> mstep s u.
-Proof.  move=> st. elim=> //{u} u v _. exact: mstep_step. Qed.
+Proof. intros st tu. revert s st. induction tu; eauto using mstep_step. Qed.
 
 Lemma mstep_lam G A B (s t : tm (A :: G) B) :
   mstep s t -> mstep (lam s) (lam t).
-Proof.
-  elim=>//{t}t u _ ih st. apply: mstep_step ih _. exact: step_abs.
-Qed.
+Proof. induction 1; eauto using mstep_step, step_abs. Qed.
 
 Lemma mstep_app G1 A B (s1 s2 : tm G1 (Fun A B)) (t1 t2 : tm G1 A) :
   mstep s1 s2 -> mstep t1 t2 -> mstep (app s1 t1) (app s2 t2).
 Proof with eauto using @mstep, @step.
-  move=> ms. elim. elim: ms... move=> {t2} t2 t3 _ ih st...
+  intros ms. induction 1. induction ms... auto...
 Qed.
 
 Lemma mstep_inl G1 A B (s1 s2: tm G1 A):
@@ -124,34 +118,28 @@ Proof.
     eapply mstep_step; eauto using mstep_refl, mstep_trans, step_orelimR.
 Qed.
 
-
 Lemma mstep_inst G1 G2 A (f : subst G1 G2) (s t : tm G1 A) :
   mstep s t -> mstep (inst f s) (inst f t).
-Proof.
-  elim=>//{t} t u _ ih st. apply: mstep_step ih _. exact: step_inst.
-Qed.
+Proof. induction 1; eauto using mstep_step, step_inst. Qed.
 
 Lemma mstep_subst G1 G2 A (f g : subst G1 G2) (s t : tm G1 A) :
   mstep s t -> (forall B i, mstep (f B i) (g B i)) ->
   mstep (inst f s) (inst g t).
 Proof with eauto using @mstep, @step.
-  move=> st1 st2. apply: mstep_trans (mstep_inst f st1) _ => {st1 s}.
-  elim: t G2 f g st2; eauto using mstep_inl, mstep_inr, mstep_app, mstep_orelim.
-  - move=> {G1 A} G1 A B s ih G2 f g st2 /=. apply: mstep_lam.
-    apply: ih => {B s} B /=[E|i]; first by destruct E.
-    rewrite/=/scomp !rinst_inst. apply: mstep_inst. exact: st2.
-  - intros. simpl. apply: mstep_orelim.
-    + now apply H.
-    + eapply H0. intros D [|]. subst. auto.
-      rewrite/=/scomp !rinst_inst. apply: mstep_inst. apply st2.
-    + eapply H1. intros D [|]. subst. auto.
-      rewrite/=/scomp !rinst_inst. apply: mstep_inst. apply st2.
+  intros st fg. apply mstep_trans with (t := inst f t); [eauto using mstep_inst|].
+  clear s st. revert G2 f g fg.
+  induction t; eauto using mstep_inl, mstep_inr, mstep_app, mstep_orelim; intros; simpl.
+  - apply mstep_lam. apply IHt. intros C [->|i]; [constructor|].
+    unfold up, scomp. rewrite !rinst_inst. apply mstep_inst, fg.
+  - apply mstep_orelim; [now apply IHt1 |apply IHt2|apply IHt3].
+    + intros D [->|i]; [constructor|]. unfold up, scomp. rewrite !rinst_inst. apply mstep_inst, fg.
+    + intros D [->|i]; [constructor|]. unfold up, scomp. rewrite !rinst_inst. apply mstep_inst, fg.
 Qed.
 
 Lemma mstep_beta G A B (s1 s2 : tm (A :: G) B) (t1 t2 : tm G A) :
   mstep s1 s2 -> mstep t1 t2 ->
   mstep (inst (t1 .: ids) s1) (inst (t2 .: ids) s2).
 Proof.
-  move=> st1 st2. apply: mstep_subst st1 _ => {B s1 s2} B /=[E|i]//.
-  by destruct E.
+  intros st1 st2. apply mstep_subst; [assumption|].
+  now intros C [->|i].
 Qed.
