coq/well-typed/reduction.v
@@ -15,39 +15,37 @@ Definition ImPred {T1 T2} (P : T1 -> Prop) (f : T1 -> T2) (y : T2) :=
   exists2 x : T1, P x & f x = y.
 
 Notation "[ 'Pred' s | x 'in' P ]" :=
-  (ImPred (fun x => P) (fun x => s)) : form_scope.
+  (ImPred (fun x => P) (fun x => s)) .
 Notation "x ∈ P" := (P x) (at level 30, only parsing).
 
 Ltac inv H := dependent destruction H.
 
 Lemma im_predI {T1 T2} (P : T1 -> Prop) (f : T1 -> T2) (x : T1) :
   P x -> f x ∈ [Pred f x' | x' in P x'].
-Proof. move=> px. by exists x. Qed.
+Proof. intros px. now exists x. Qed.
 
 Lemma step_weak {G1 G2 A} (f : ren G1 G2) (s : tm G1 A) (t : tm G2 A) :
   step (rinst f s) t -> t ∈ [Pred rinst f s' | s' in step s s'].
-Proof.
-  move=> st. dependent induction st.
-  - inv s => //. inv x. inv s1 => //. inv x.
-    rewrite !rinst_inst. fsimpl. rewrite inst_up_beta. rewrite -rinst_inst.
-    apply: im_predI. exact: step_beta.
-  - inv s => //. inv x. case: (IHst _ _ _ erefl) => {IHst} s' ih e.
-    exists (lam s'). by constructor. by rewrite -e.
-  - inv s => //. inv x. case: (IHst _ _ _ erefl) => {IHst} s' ih e.
-    exists (app s' s4). by constructor. by rewrite -e.
-  - inv s => //. inv x. case: (IHst _ _ _ erefl) => {IHst} s' ih e.
-    exists (app s1 s'). by constructor. by rewrite -e.
+Proof with simpl in *; try congruence.
+  intros st. dependent induction st.
+  - inv s... inv s1; try inv x... asimpl.
+    eexists. constructor. now asimpl.
+  - inv s... inv x. destruct (IHst _ _ _ eq_refl) as [s' ih <-].
+    exists (lam s'). now constructor. now fsimpl.
+  - inv s... inv x. destruct (IHst _ _ _ eq_refl) as [s' ih <-].
+    exists (app s' s4). now constructor. now fsimpl.
+  - inv s... inv x. destruct (IHst _ _ _ eq_refl) as [s' ih <-].
+    exists (app s1 s'). now constructor. now fsimpl.
 Qed.
 
 Lemma step_inst {G1 G2 A} (f : subst G1 G2) (s t : tm G1 A) :
   step s t -> step (inst f s) (inst f t).
 Proof.
-  move=> st. elim: st G2 f => {G1 A s t}
-    [G1 A B b t|G1 A B b1 b2 _ ih|G1 A B s1 s2 t _ ih|G1 A B s t1 t2 _ ih] G2 f/=.
-  - rewrite -inst_up_beta. exact: step_beta.
-  - apply: step_abs. exact: ih.
-  - apply: step_appL. exact: ih.
-  - apply: step_appR. exact: ih.
+  intros st. revert G2 f. induction st as  [G1 A B b t|G1 A B b1 b2 _ ih|G1 A B s1 s2 t _ ih|G1 A B s t1 t2 _ ih]; intros G2 f; cbn.
+  - rewrite <- inst_up_beta. apply step_beta.
+  - apply step_abs, ih.
+  - apply step_appL, ih.
+  - apply step_appR, ih.
 Qed.
 
 (** ** Multi-step reduction *)
@@ -57,39 +55,37 @@ Inductive mstep {G A} (s : tm G A) : tm G A -> Prop :=
 Hint Resolve mstep_refl.
 
 Lemma mstep_trans G A (s t u : tm G A) : mstep s t -> mstep t u -> mstep s u.
-Proof. move=> st. elim=> //{u} u v _. exact: mstep_step. Qed.
+Proof. intros st tu. revert s st. induction tu; eauto using mstep_step. Qed.
 
 Lemma mstep_lam G A B (s t : tm (A :: G) B) :
   mstep s t -> mstep (lam s) (lam t).
-Proof. elim=>//{t}t u _ ih st. apply: mstep_step ih _. exact: step_abs. Qed.
+Proof. induction 1; eauto using mstep_step, step_abs. Qed.
 
 Lemma mstep_app G1 A B (s1 s2 : tm G1 (Fun A B)) (t1 t2 : tm G1 A) :
   mstep s1 s2 -> mstep t1 t2 -> mstep (app s1 t1) (app s2 t2).
 Proof with eauto using @mstep, @step.
-  move=> ms. elim. elim: ms... move=> {t2} t2 t3 _ ih st...
+  intros ms. induction 1. induction ms... auto...
 Qed.
 
 Lemma mstep_inst G1 G2 A (f : subst G1 G2) (s t : tm G1 A) :
   mstep s t -> mstep (inst f s) (inst f t).
-Proof.  elim=>//{t} t u _ ih st. apply: mstep_step ih _. exact: step_inst. Qed.
+Proof. induction 1; eauto using mstep_step, step_inst. Qed.
 
 Lemma mstep_subst G1 G2 A (f g : subst G1 G2) (s t : tm G1 A) :
   mstep s t -> (forall B i, mstep (f B i) (g B i)) ->
   mstep (inst f s) (inst g t).
 Proof with eauto using @mstep, @step.
-  move=> st1 st2. apply: mstep_trans (mstep_inst f st1) _ => {st1 s}.
-  elim: t G2 f g st2...
-  - move=> {G1 A} G1 A B s ihs t iht G2 f g st2 /=. apply: mstep_app.
-    exact: ihs. exact: iht.
-  - move=> {G1 A} G1 A B s ih G2 f g st2 /=. apply: mstep_lam.
-    apply: ih => {B s} B /=[E|i]; first by destruct E.
-    rewrite/=/scomp !rinst_inst. apply: mstep_inst. exact: st2.
+  intros st fg. apply mstep_trans with (t := inst f t); [eauto using mstep_inst|].
+  clear s st. revert G2 f g fg.
+  induction t; eauto using mstep_app; intros; simpl.
+  - apply mstep_lam. apply IHt. intros C [->|i]; [constructor|].
+    unfold up, scomp. rewrite !rinst_inst. apply mstep_inst, fg.
 Qed.
 
 Lemma mstep_beta G A B (s1 s2 : tm (A :: G) B) (t1 t2 : tm G A) :
   mstep s1 s2 -> mstep t1 t2 ->
   mstep (inst (t1 .: ids) s1) (inst (t2 .: ids) s2).
 Proof.
-  move=> st1 st2. apply: mstep_subst st1 _ => {B s1 s2} B /=[E|i]//.
-  by destruct E.
+  intros st1 st2. apply mstep_subst; [assumption|].
+  now intros C [->|i].
 Qed.
