coq/well-typed/sn_inductive_2a.v
@@ -20,7 +20,7 @@ Proof.
     eauto using SRed.
   - exists (inst (M'0_2 .: ids) M'0_1).
     split. now asimpl. eauto using SNRed.
-  - destruct (H0 _ _ _ (erefl (rinst R0 M'1))) as (N'&->&A2).
+  - destruct (H0 _ _ _ (eq_refl (rinst R0 M'1))) as (N'&->&A2).
     exists (app N' M'2). split; [reflexivity| now constructor].
 Qed.
 
